doc/coq/simple/Linking.v
@@ -1,577 +1,207 @@
-From Simple Require Export Sound.
-Require Export Coq.Logic.FunctionalExtensionality.
+From Simple Require Export Concrete.
 
 Generalizable Variables T BT AT.
 
-Definition inject_ctx_mem `{Eq T} (Cout : @dy_ctx T) (mem : T -> option expr_value) :=
-  fun t => match mem t with None => None | Some v => Some (inject_ctx_v Cout v) end.
-
-Definition delete_ctx_mem `{Eq T} `{Eq AT} (α : T -> AT) (Cout : @dy_ctx T) (mem : T -> option expr_value) :=
-  let eqb' t t' := eqb (α t) (α t') in
-  fun t => match mem t with None => None | Some v => Some (delete_ctx_v eqb' Cout v) end.
-
-Lemma delete_ctx_mem_eq `{Eq T} `{Eq AT} (α : T -> AT) :
-  forall (Cout : @dy_ctx T) (mem : T -> option expr_value),
-         delete_ctx_mem α Cout (inject_ctx_mem Cout mem) = mem.
-Proof.
-  intros. apply functional_extensionality.
-  intros. unfold inject_ctx_mem. unfold delete_ctx_mem.
-  destruct (mem x); eauto.
-  simpl. destruct e; simpl; rewrite delete_inject_eq.
-  eauto. intros. rewrite eqb_eq. eauto.
-Qed.
-
-Inductive link {BT AT} (final : BT) (init : AT) :=
-  | L (bf : BT) (af : AT)
-. 
-
-Definition link_eqb `{Eq BT} `{Eq AT} (final : BT) (init : AT)
-  (t1 : link final init) (t2 : link final init) :=
+Definition link_leb `{TotalOrder BT} `{TotalOrder AT}
+  (t1 : link BT AT) (t2 : link BT AT) :=
   match t1, t2 with
-  | L _ _ bf af, L _ _ bf' af' =>
-    eqb bf bf' && eqb af af'
+  | BF t1, BF t2 => leb t1 t2
+  | AF t1, AF t2 => leb t1 t2
+  | BF _, AF _ => true
+  | AF _, BF _ => false
   end.
 
-Definition link_leb `{OrderT BT} `{OrderT AT} (final : BT) (init : AT) 
-  (t1 : link final init) (t2 : link final init) :=
-  match t1, t2 with
-  | L _ _ bf af, L _ _ bf' af' =>
-    if leb bf bf' then
-      if eqb bf bf' then
-        leb af af'
-      else true
-    else false
-  end.
-
-Lemma link_leb_refl `{OrderT BT} `{OrderT AT} (final : BT) (init : AT) : 
-  forall t, link_leb final init t t = true.
+Lemma link_leb_refl `{TotalOrder BT} `{TotalOrder AT} : 
+  forall (t : link BT AT), link_leb t t = true.
 Proof.
-  intros. destruct t. simpl. rewrite leb_refl. 
-  replace (eqb bf bf) with true.
-  apply leb_refl.
-  symmetry. apply eqb_eq. eauto.
+  intros. destruct t; simpl; rewrite leb_refl; eauto.
 Qed.
 
-Lemma link_leb_trans `{OrderT BT} `{OrderT AT} (final : BT) (init : AT) :
-  forall t t' t''
-    (LE : link_leb final init t t' = true)
-    (LE' : link_leb final init t' t'' = true),
-  link_leb final init t t'' = true.
+Lemma link_leb_trans `{TotalOrder BT} `{TotalOrder AT} :
+  forall (t t' t'' : link BT AT)
+    (LE : link_leb t t' = true)
+    (LE' : link_leb t' t'' = true),
+  link_leb t t'' = true.
 Proof.
   intros.
-  destruct t as [bf af]; destruct t' as [bf' af'];
-  destruct t'' as [bf'' af'']; simpl in *.
-  destruct (leb bf bf') eqn:LEbf;
-  destruct (leb bf' bf'') eqn:LEbf';
-  try (inversion LE; fail);
-  try (inversion LE'; fail).
-  - destruct (eqb bf bf') eqn:EQbf;
-    destruct (eqb bf' bf'') eqn:EQbf';
-    try rewrite eqb_eq in *;
-    try rewrite eqb_neq in *;
-    replace (leb bf bf'') with true;
-    try (symmetry; apply leb_trans with (t' := bf'); eauto).
-    replace (eqb bf bf'') with true.
-    apply leb_trans with (t' := af'); eauto.
-    symmetry. apply eqb_eq; subst; eauto.
-    replace (eqb bf bf'') with false. eauto.
-    symmetry. apply eqb_neq. red. intros. subst.
-    apply EQbf'. eauto.
-    replace (eqb bf bf'') with false. eauto.
-    symmetry. apply eqb_neq. red. intros. subst.
-    apply EQbf. eauto.
-    replace (eqb bf bf'') with false. eauto.
-    symmetry. apply eqb_neq. red. intros. subst.
-    apply EQbf. apply leb_sym; eauto.
+  unfold link_leb in *;
+  repeat des_goal; repeat des_hyp; clarify;
+  eapply leb_trans; eauto.
 Qed.
 
-Lemma link_leb_sym `{OrderT BT} `{OrderT AT} (final : BT) (init : AT) :
-  forall t t'
-    (LE : link_leb final init t t' = true)
-    (LE' : link_leb final init t' t = true),
+Lemma link_leb_sym `{TotalOrder BT} `{TotalOrder AT} :
+  forall (t t' : link BT AT)
+    (LE : link_leb t t' = true)
+    (LE' : link_leb t' t = true),
   t = t'.
 Proof.
   intros.
-  destruct t as [bf af]; destruct t' as [bf' af'];
-  simpl in *;
-  destruct (leb bf bf') eqn:LEbf;
-  destruct (leb bf' bf) eqn:LEbf';
-  try (inversion LE; fail);
-  try (inversion LE'; fail).
-  assert (bf' = bf) as RR.
-  apply leb_sym; eauto.
-  rewrite RR in *.
-  replace (eqb bf bf) with true in *.
-  assert (af = af').
-  apply leb_sym; eauto. subst; eauto.
-  symmetry. apply eqb_eq. eauto.
+  unfold link_leb in *.
+  repeat des_hyp; clarify;
+  match goal with
+  | |- BF ?t = BF ?t' =>
+    assert (t = t'); 
+    first [solve [subst; eauto] | apply leb_sym; auto]
+  | |- AF ?t = AF ?t' => 
+    assert (t = t');
+    first [solve [subst; eauto] | apply leb_sym; auto]
+  end.
 Qed.
 
-Lemma link_leb_or `{OrderT BT} `{OrderT AT} (final : BT) (init : AT) :
-  forall t t',
-  let le1 := link_leb final init t t' in
-  let le2 := link_leb final init t' t in
-  le1 || le2 = true.
+Lemma link_leb_or `{TotalOrder BT} `{TotalOrder AT} :
+  forall (t t' : link BT AT),
+  (link_leb t t') || (link_leb t' t) = true.
 Proof.
   intros.
-  destruct t as [bf af]; destruct t' as [bf' af'].
-  simpl in *.
-  destruct (leb bf bf') eqn:LEbf;
-  destruct (leb bf' bf) eqn:LEbf';
-  subst le1 le2.
-  - replace bf with bf'; try (apply leb_sym; eauto).
-    rewrite t_refl. apply leb_or.
-  - assert (eqb bf bf' = false) as RR.
-    { refl_bool. intros contra.
-      rewrite eqb_eq in contra. subst.
-      rewrite leb_refl in LEbf'. inversion LEbf'. }
-    rewrite RR. eauto.
-  - assert (eqb bf' bf = false) as RR.
-    { refl_bool. intros contra.
-      rewrite eqb_eq in contra. subst.
-      rewrite leb_refl in LEbf. inversion LEbf. }
-    rewrite RR. eauto.
-  - assert (leb bf bf' || leb bf' bf = true) as contra.
-    apply leb_or. rewrite LEbf in contra. rewrite LEbf' in contra.
-    inversion contra.
+  unfold link_leb in *.
+  repeat des_goal; repeat des_hyp; clarify;
+  match goal with
+  | _ : AT,
+    RR : leb ?a ?b = false 
+    |- leb ?b ?a = true =>
+    pose proof (@leb_or AT _ _ a b);
+    rewrite RR in *
+  | _ : BT,
+    RR : leb ?a ?b = false 
+    |- leb ?b ?a = true =>
+    pose proof (@leb_or BT _ _ a b);
+    rewrite RR in *
+  end; ss.
 Qed.
 
-Lemma link_eqb_eq `{Eq BT} `{Eq AT} (final : BT) (init : AT):
-  forall t t', link_eqb final init t t' = true <-> t = t'.
-Proof.
-  intros.
-  destruct t as [bf af]; destruct t' as [bf' af'];
-  simpl in *;
-  split; intro EQ.
-  destruct (eqb bf bf') eqn:EQbf;
-  destruct (eqb af af') eqn:EQaf;
-  try (inversion EQ; fail).
-  rewrite eqb_eq in EQbf.
-  rewrite eqb_eq in EQaf. subst. eauto.
-  inversion EQ; subst.
-  repeat rewrite t_refl. eauto.
-Qed.
-
-Lemma link_eqb_neq `{Eq BT} `{Eq AT} (final : BT) (init : AT):
-  forall t t', link_eqb final init t t' = false <-> t <> t'.
-Proof.
-  intros.
-  split; intro NEQ.
-  red. intros EQ.
-  assert (link_eqb final init t t' = true) as RR. apply link_eqb_eq. eauto.
-  rewrite RR in NEQ. inversion NEQ.
-  refl_bool. intros contra. rewrite link_eqb_eq in contra.
-  apply NEQ; eauto.
-Qed.
-
-#[export] Instance LinkEq `{Eq BT} `{Eq AT} (final : BT) (init : AT) :
-  Eq (link final init) :=
-{
-  eqb := link_eqb final init;
-  eqb_eq := link_eqb_eq final init;
-  eqb_neq := link_eqb_neq final init
-}.
-
-#[export] Instance LinkOrderT `{OrderT BT} `{OrderT AT} (final : BT) (init : AT) :
-  @OrderT (link final init) (LinkEq final init) :=
+#[export] Instance LinkOrder `{TotalOrder BT} `{TotalOrder AT} :
+  @TotalOrder (link BT AT) (@link_eq BT _ AT _) :=
   {
-    leb := link_leb final init;
-    leb_refl := link_leb_refl final init;
-    leb_trans := link_leb_trans final init;
-    leb_sym := link_leb_sym final init;
-    leb_or := link_leb_or final init
+    leb := link_leb;
+    leb_refl := link_leb_refl;
+    leb_trans := link_leb_trans;
+    leb_sym := link_leb_sym;
+    leb_or := link_leb_or;
   }.
 
-Fixpoint filter_ctx_bf
-  `{OrderT BT} `{EA : Eq AT} (final : BT) (init : AT)
-  (C : @dy_ctx (link final init)) :=
-  match C with
-  | ([||]) => ([||])
-  | dy_binde x (L _ _ bf af) C' =>
-    let filtered := filter_ctx_bf final init C' in
-    if eqb final bf then filtered else dy_binde x bf filtered
-  | dy_bindm M C' C'' =>
-    dy_bindm M (filter_ctx_bf final init C') (filter_ctx_bf final init C'')
-  end.
-
-Fixpoint filter_ctx_af
-  `{OrderT BT} `{EA : Eq AT} (final : BT) (init : AT)
-  (C : @dy_ctx (link final init)) :=
-  match C with
-  | ([||]) => ([||])
-  | dy_binde x (L _ _ bf af) C' =>
-    let filtered := filter_ctx_af final init C' in
-    if eqb final bf then dy_binde x af filtered else filtered
-  | dy_bindm M C' C'' =>
-    dy_bindm M (filter_ctx_af final init C') (filter_ctx_af final init C'')
-  end.
-
-Definition filter_v_bf 
-  `{OrderT BT} `{EA : Eq AT} (final : BT) (init : AT)
-  (v : @expr_value (link final init)) :=
-  match v with
-  | Closure x e C => Closure x e (filter_ctx_bf final init C)
-  end.
-
-Definition filter_v_af
-  `{OrderT BT} `{EA : Eq AT} (final : BT) (init : AT)
-  (v : @expr_value (link final init)) :=
-  match v with
-  | Closure x e C => Closure x e (filter_ctx_af final init C)
-  end.
-
-Definition filter_mem_bf
-  `{OrderT BT} `{EA : Eq AT} (final : BT) (init : AT)
-  (mem : (link final init) -> option (@expr_value (link final init))) :=
-  fun t =>
-    match mem (L _ _ t init) with
-    | Some v => Some (filter_v_bf final init v)
-    | None => None
-    end.
-
-Definition filter_mem_af
-  `{OrderT BT} `{EA : Eq AT} (final : BT) (init : AT)
-  (mem : (link final init) -> option (@expr_value (link final init))) :=
-  fun t =>
-    match mem (L _ _ final t) with
-    | Some v => Some (filter_v_af final init v)
-    | None => None
-    end.
-
-Fixpoint lift_ctx_bf `{Eq BT} `{Eq AT} (final : BT) (init : AT) (C : @dy_ctx BT)
-  : @dy_ctx (link final init) :=
-  match C with
-  | ([||]) => ([||])
-  | dy_binde x t C' => dy_binde x (L _ _ t init) (lift_ctx_bf final init C')
-  | dy_bindm M C' C'' => dy_bindm M (lift_ctx_bf final init C') (lift_ctx_bf final init C'')
-  end.
-
-Fixpoint lift_ctx_af `{Eq BT} `{Eq AT} (final : BT) (init : AT) (C : @dy_ctx AT)
-  : @dy_ctx (link final init) :=
-  match C with
-  | ([||]) => ([||])
-  | dy_binde x t C' => dy_binde x (L _ _ final t) (lift_ctx_af final init C')
-  | dy_bindm M C' C'' => dy_bindm M (lift_ctx_af final init C') (lift_ctx_af final init C'')
-  end.
-
-Definition lift_v_af `{Eq BT} `{Eq AT} (final : BT) (init : AT) (v : @expr_value AT)
-  : @expr_value (link final init) :=
-  match v with
-  | Closure x e C => Closure x e (lift_ctx_af final init C)
-  end.
-
-Definition link_tick `{time BT} `{time AT} (final : BT) (init : AT) (Cout : @dy_ctx BT)
-  `{Eq T} (α : link final init -> T)
-  C st x v :=
-  match st with
-  | ST mem (L _ _ bf af) =>
-    if eqb final bf then
-      let Cout := lift_ctx_bf final init Cout in
-      let eqb' t t' := eqb (α t) (α t') in
-      let af' := 
-        tick (filter_ctx_af final init (delete_ctx eqb' Cout C))
-             (ST (filter_mem_af final init (delete_ctx_mem α Cout mem)) af)
-             x (filter_v_af final init (delete_ctx_v eqb' Cout v)) in
-      L final init final af'
-    else
-      let bf' := tick (filter_ctx_bf final init C)
-                      (ST (filter_mem_bf final init mem) bf)
-                      x (filter_v_bf final init v)
-      in L final init bf' init
-  end.
-
-Lemma link_tick_lt `{time BT} `{time AT} (final : BT) (init : AT) (Cout : @dy_ctx BT)
-  `{Eq T} (α : link final init -> T):
-  forall C mem t x v, t < link_tick final init Cout α C (ST mem t) x v.
-Proof.
-  destruct t; unfold "<"; simpl.
-  destruct (eqb final bf) eqn:EQ; simpl;
-  try rewrite eqb_eq in EQ; try rewrite eqb_neq in EQ.
-  - intros. subst. rewrite leb_refl. rewrite t_refl. simpl.
-    split; try apply tick_lt.
-  - intros.
-    destruct (leb
-      (tick (filter_ctx_bf final init C)
-         (ST (filter_mem_bf final init mem) bf) x 
-         (filter_v_bf final init v)) final) eqn:LT; simpl.
-    + replace (leb bf
-      (tick (filter_ctx_bf final init C) (ST (filter_mem_bf final init mem) bf)
-        x (filter_v_bf final init v))) with true; try (symmetry; apply tick_lt).
-      replace (eqb bf
-      (tick (filter_ctx_bf final init C) (ST (filter_mem_bf final init mem) bf)
-        x (filter_v_bf final init v))) with false; try (symmetry; apply tick_lt).
-      eauto.
-    + replace (leb bf
-      (tick (filter_ctx_bf final init C) (ST (filter_mem_bf final init mem) bf)
-        x (filter_v_bf final init v))) with true; try (symmetry; apply tick_lt).
-      replace (eqb bf
-      (tick (filter_ctx_bf final init C) (ST (filter_mem_bf final init mem) bf)
-        x (filter_v_bf final init v))) with false; try (symmetry; apply tick_lt).
-      eauto.
-Qed.
-
-#[export] Instance link_time `{time BT} `{time AT} `{Eq T}
-  (final : BT) (init : AT) (Cout : @dy_ctx BT) (α : link final init -> T) : (@time (link final init) _ _) :=
-  {
-    tick := link_tick final init Cout α;
-    tick_lt := link_tick_lt final init Cout α
-  }.
-
-Definition link_mem `{OrderT BT} `{Eq AT}
-  (bmem : BT -> option (@expr_value BT)) (final : BT) (init : AT) (Cout : @dy_ctx BT)
-  (amem : AT -> option (@expr_value AT)) : (link final init) -> option expr_value :=
-  fun t =>
+Definition link_tick `{Eq T} `{time BT} `{time AT} (Cout : dy_ctx BT) 
+  (α : link BT AT -> T) :=
+  let eqb t t' := eqb (α t) (α t') in
+  fun C m t x v =>
     match t with
-    | L _ _ bf af =>
-      if eqb final bf then
-        let Cout := lift_ctx_bf final init Cout in
-        match amem af with
-        | Some (Closure x e C) => Some (Closure x e (Cout<|lift_ctx_af final init C|>))
-        | None => None
-        end
-      else match bmem bf with
-        | Some (Closure x e C) => Some (Closure x e (lift_ctx_bf final init C))
-        | None => None
-        end
+    | BF t => BF (tick (filter_ctx_bf C) (filter_mem_bf m) t x (filter_v_bf v))
+    | AF t =>
+      let Cout := lift_ctx_bf Cout in
+      AF (tick (filter_ctx_af (delete eqb Cout C))
+            (filter_mem_af (delete_ctx_mem eqb Cout m)) t
+            x (filter_v_af (delete_v eqb Cout v)))
     end.
 
-Lemma filter_lift_eq_af `{time BT} `{time AT} (final : BT) (init : AT):
-  forall (C : @dy_ctx AT),
-    filter_ctx_af final init (lift_ctx_af final init C) = C.
+Local Lemma t_refl `{Eq T} {TT} (α : TT -> T) :
+  forall t, 
+  let eqb t t' := eqb (α t) (α t') in
+  eqb t t = true.
 Proof.
-  induction C; simpl; try rewrite IHC; try rewrite t_refl; eauto.
-  rewrite IHC2. rewrite IHC1. eauto.
+  ii; subst eqb; ss; rewrite eqb_eq; eauto.
 Qed.
 
-Lemma filter_lift_eq_bf `{time BT} `{time AT} (final : BT) (init : AT) :
-  forall (C : @dy_ctx BT) (BOUND : dy_ctx_bound C final),
-    filter_ctx_bf final init (lift_ctx_bf final init C) = C.
+Lemma link_tick_ext `{Eq T} `{time BT} `{time AT} (Cout : dy_ctx BT) (α : link BT AT -> T) :
+  forall C m m' t x v (SAME : same m m'),
+  link_tick Cout α C m t x v = link_tick Cout α C m' t x v.
 Proof.
-  induction C; intros; simpl in *;
-  try rewrite IHC; try apply BOUND;
-  try replace (eqb final tx) with false; eauto;
-  try destruct BOUND as [[LE NEQ] BOUND];
-  try (symmetry; refl_bool; intros contra;
-      rewrite eqb_eq in contra; subst; rewrite t_refl in NEQ; inversion NEQ).
-  rewrite IHC2; try rewrite IHC1; eauto; apply BOUND.
+  intros. destruct t; simpl;
+  match goal with
+  | |- BF ?a = BF ?b =>
+    assert (a = b) as RR;
+    first [rewrite RR; reflexivity | apply tick_ext]
+  | |- AF ?a = AF ?b =>
+    assert (a = b) as RR;
+    first [rewrite RR; reflexivity | apply tick_ext]
+  end; unfold same in *; ii;
+  match goal with
+  | |- Some ?v = read (filter_mem_bf _) ?t <-> _ =>
+    specialize (SAME (BF t));
+    repeat rewrite read_filter_bf;
+    split; i; des; clarify; eexists; split;
+    try reflexivity; rewrite SAME in *; assumption
+  | |- Some ?v = read (filter_mem_af _) ?t <-> _ =>
+    specialize (SAME (AF t));
+    repeat rewrite read_filter_af;
+    split; i; des; clarify; eexists; split;
+    try reflexivity; rewrite read_delete in *;
+    des; clarify; eexists; split;
+    try reflexivity; rewrite SAME in *; assumption
+  end.
 Qed.
 
-Lemma filter_delete_eq `{time BT} `{time AT} `{Eq T} (final : BT) (init : AT) (Cout : @dy_ctx BT) (α : link final init -> T) :
-  forall bmem amem,
-  filter_mem_af final init
-    (delete_ctx_mem α (lift_ctx_bf final init Cout)
-    (link_mem bmem final init Cout amem)) = amem.
+Lemma link_tick_lt `{Eq T} `{time BT} `{time AT} (Cout : dy_ctx BT) (α : link BT AT -> T) :
+  forall C m t x v, t < link_tick Cout α C m t x v.
 Proof.
-  intros. apply functional_extensionality.
-  intros. unfold filter_mem_af.
-  unfold delete_ctx_mem. simpl. rewrite t_refl.
-  remember (lift_ctx_bf final init Cout) as vout eqn:E. clear E.
-  remember (amem x) as o eqn:E. clear E.
-  destruct o; eauto. destruct e. simpl.
-  rewrite delete_inject_eq. rewrite filter_lift_eq_af. eauto.
-  intros. rewrite eqb_eq. eauto.
+  destruct t; ss; ii; unfold "<"; s; apply tick_lt.
 Qed.
 
-Lemma link_tick_eq `{time BT} `{time AT} `{Eq T} (final : BT) (init : AT) (Cout : @dy_ctx BT) (α : link final init -> T) :
+#[export] Instance link_time `{Eq T} `{time BT} `{time AT}
+  (Cout : dy_ctx BT) (α : link BT AT -> T) : (@time (link BT AT) _ _) :=
+  {
+    tick := link_tick Cout α;
+    tick_lt := link_tick_lt Cout α;
+    tick_ext := link_tick_ext Cout α;
+  }.
+
+Lemma link_tick_eq `{Eq T} `{time BT} `{time AT} (Cout : dy_ctx BT) (α : link BT AT -> T) :
   forall bmem C amem t x v,
-    link_tick final init Cout α ((lift_ctx_bf final init Cout)<|(lift_ctx_af final init C)|>)
-              (ST (link_mem bmem final init Cout amem) (L final init final t)) x 
-              (inject_ctx_v (lift_ctx_bf final init Cout) (lift_v_af final init v)) =
-    L final init final (tick C (ST amem t) x v).
+    link_tick Cout α ((lift_ctx_af C)[|(lift_ctx_bf Cout)|])
+          (link_mem bmem Cout amem) (AF t) x 
+          (inject_v (lift_ctx_bf Cout) (lift_v_af v)) =
+    AF (tick C amem t x v).
 Proof.
-  intros. destruct v. unfold inject_ctx_v. simpl.
-  rewrite delete_inject_eq; try (intros; rewrite eqb_eq; eauto).
-  rewrite delete_inject_eq; try (intros; rewrite eqb_eq; eauto).
+  intros. destruct v. unfold inject_v. simpl.
+  repeat rewrite delete_inject_eq.
   rewrite filter_delete_eq.
-  rewrite filter_lift_eq_af. rewrite filter_lift_eq_af. rewrite t_refl.
+  rewrite filter_lift_eq_af. rewrite filter_lift_eq_af.
   reflexivity.
+  all:(apply t_refl).
 Qed.
 
-Lemma link_update_m_eq `{time BT} `{time AT} (final : BT) (init : AT) (Cout : @dy_ctx BT) :
-  forall bmem amem t v (BOUND : time_bound Cout (ST bmem final)),
-  (L final init final t !-> inject_ctx_v (lift_ctx_bf final init Cout) (lift_v_af final init v);
-    (link_mem bmem final init Cout amem)) =
-    link_mem bmem final init Cout (t !-> v; amem).
+Lemma link_eval_eq `{Eq T} `{time BT} `{time AT}
+  (Cout : dy_ctx BT) (α : link BT AT -> T) :
+  forall bmem e (C : dy_ctx AT) m t cf' (EVAL : {|(Cf e C m t) ~> cf'|}),
+  (@step (link BT AT) _ _ (@link_time T _ BT _ _ _ AT _ _ _ Cout α) (inject_cf Cout bmem (Cf e C m t)) (inject_cf Cout bmem cf')).
 Proof.
-  intros. apply functional_extensionality.
-  intros. unfold update_m. destruct v. simpl.
-  destruct x; simpl; eauto.
-  destruct (eqb bf final) eqn:EQb; destruct (eqb af t) eqn:EQa; simpl; eauto.
-  rewrite eqb_eq in EQb. rewrite eqb_eq in EQa.
-  subst. rewrite t_refl. eauto.
-  destruct (eqb final bf) eqn:EQb'; eauto.
-  rewrite eqb_eq in EQb'. subst.
-  rewrite eqb_neq in EQb. contradict.
-Qed.
-
-Lemma lift_addr_x `{time BT} `{time AT} (final : BT) (init :AT) :
-  forall (C : @dy_ctx AT) x,
-    addr_x (lift_ctx_af final init C) x =
-      match addr_x C x with
-      | Some addr => Some (L final init final addr)
-      | None => None
-      end.
-Proof.
-  induction C; simpl; eauto;
-  intros;
-  destruct (eq_eid x0 x); rewrite IHC;
-  destruct (addr_x C x0); eauto.
-Qed.
-
-Lemma lift_ctx_M `{time BT} `{time AT} (final : BT) (init : AT) :
-  forall (C : @dy_ctx AT) M,
-    ctx_M (lift_ctx_af final init C) M =
-      match ctx_M C M with
-      | Some CM => Some (lift_ctx_af final init CM)
-      | None => None
-      end.
-Proof.
-  induction C; simpl; eauto;
-  intros.
-  destruct (eq_mid M0 M); rewrite IHC2;
-  destruct (ctx_M C2 M0); eauto.
-Qed.
-
-Lemma lift_plugin_af `{time BT} `{time AT} (final : BT) (init : AT) :
-  forall (C C' : @dy_ctx AT),
-    lift_ctx_af final init (C[|C'|]) = (lift_ctx_af final init C [|lift_ctx_af final init C'|]).
-Proof.
-  induction C; simpl; intros; try rewrite IHC; eauto.
-  rewrite IHC2. eauto.
-Qed.
-
-Lemma link_eval_eq `{time BT} `{time AT} `{Eq T}
-  (final : BT) (init : AT) (Cout : @dy_ctx BT) (α : link final init -> T) :
-  forall bmem (BOUND : time_bound Cout (ST bmem final))
-         C st e v st'
-         (EVAL : @EvalR AT _ _ _ C st e v st'),
-    let inject_C := (lift_ctx_bf final init Cout) <|(lift_ctx_af final init C)|> in
-    let inject_v :=
-      match v with
-      | EVal ev => EVal (inject_ctx_v (lift_ctx_bf final init Cout) (lift_v_af final init ev))
-      | MVal C_v => MVal ((lift_ctx_bf final init Cout)<|(lift_ctx_af final init C_v)|>)
-      end in
-    let inject_st :=
-      match st with
-      | ST amem t => ST (link_mem bmem final init Cout amem) (L _ _ final t)
-      end in
-    let inject_st' :=
-      match st' with
-      | ST amem' t' => ST (link_mem bmem final init Cout amem') (L _ _ final t')
-      end in
-    @EvalR (link final init) _ _ (link_time final init Cout α)
-      inject_C inject_st e inject_v inject_st'.
-Proof.
-  intros. induction EVAL;
-  try destruct v; try destruct st; try destruct st'; try destruct st'';
-  try (destruct inject_v eqn:INJv; inversion INJv; subst);
-  try (destruct inject_st eqn:INJst; inversion INJst; subst);
-  try (destruct inject_st' eqn:INJst'; inversion INJst'; subst); eauto.
-  - inversion STATE; subst.
-    eapply Eval_var_e; eauto.
-    pose proof (inject_ctx_addr_x x (lift_ctx_bf final init Cout) (lift_ctx_af final init C)) as RR.
-    rewrite lift_addr_x in RR.
-    rewrite <- ADDR in RR. symmetry. apply RR.
-    unfold link_mem. rewrite t_refl.
-    rewrite <- ACCESS. eauto.
-  - destruct st_v. destruct arg.
-    eapply Eval_app. apply IHEVAL1. apply IHEVAL2.
-    pose proof (link_tick_eq final init Cout α bmem C mem t x (Closure x1 e3 C1)) as RR.
-    simpl in *. subst inject_C.
-    rewrite RR. clear RR.
-    pose proof (link_update_m_eq final init Cout bmem mem t (Closure x1 e3 C1) BOUND) as RR. simpl in RR.
-    rewrite RR. clear RR.
-    replace (dy_binde x (L _ _ final t) ([||])) with 
-    (map_inject (lift_ctx_bf final init Cout) (dy_binde x (L _ _ final t) ([||]))) by reflexivity.
-    rewrite plugin_inject_assoc. rewrite lift_plugin_af in IHEVAL3. eauto.
-  - pose proof (inject_ctx_ctx_M M (lift_ctx_bf final init Cout) (lift_ctx_af final init C)) as RR.
-    rewrite lift_ctx_M in RR.
-    rewrite <- ACCESS in RR.
-    eapply Eval_var_m; eauto.
-  - eapply Eval_lete; eauto.
-    pose proof (link_tick_eq final init Cout α bmem C mem t x (Closure x0 e0 C0)) as RR.
-    simpl in *. subst inject_C.
-    rewrite RR. clear RR.
-    pose proof (link_update_m_eq final init Cout bmem mem t (Closure x0 e0 C0) BOUND) as RR. simpl in RR.
-    rewrite RR. clear RR.
-    replace (dy_binde x (L _ _ final t) ([||])) with 
-    (map_inject (lift_ctx_bf final init Cout) (dy_binde x (L _ _ final t) ([||]))) by reflexivity.
-    rewrite plugin_inject_assoc. rewrite lift_plugin_af in IHEVAL2. eauto.
-  - eapply Eval_letm; eauto.
-    assert (inject_C [|dy_bindm M (lift_ctx_bf final init Cout <| lift_ctx_af final init C' |>) ([||])|] =
-            (lift_ctx_bf final init Cout <| lift_ctx_af final init (C [|dy_bindm M C' ([||])|]) |>)) as RR. 
-    { subst inject_C. rewrite lift_plugin_af.
-      rewrite <- plugin_inject_assoc. simpl. eauto. } 
-    rewrite RR. clear RR. simpl in *. exact IHEVAL2.
-Qed.
-
-Lemma link_reach_eq `{time BT} `{time AT} `{Eq T}
-  (final : BT) (init : AT) (Cout : @dy_ctx BT) (α : link final init -> T) :
-  forall bmem (BOUND : time_bound Cout (ST bmem final))
-         C st e C' st' e'
-         (REACH : @one_reach AT _ _ _ C st e C' st' e'),
-    let inject_C := (lift_ctx_bf final init Cout) <|(lift_ctx_af final init C)|> in
-    let inject_C' := (lift_ctx_bf final init Cout) <|(lift_ctx_af final init C')|> in
-    let inject_st :=
-      match st with
-      | ST amem t => ST (link_mem bmem final init Cout amem) (L _ _ final t)
-      end in
-    let inject_st' :=
-      match st' with
-      | ST amem' t' => ST (link_mem bmem final init Cout amem') (L _ _ final t')
-      end in
-    @one_reach (link _ _) _ _ (link_time final init Cout α)
-      inject_C inject_st e inject_C' inject_st' e'.
-Proof.
-  intros. destruct REACH; try destruct st.
-  - apply one_appl.
-  - destruct st_lam.
-    eapply link_eval_eq with (Cout := Cout) (bmem := bmem) in FN; eauto.
-    eapply one_appr; simpl in *; eauto.
-  - eapply link_eval_eq with (Cout := Cout) (bmem := bmem) in FN; eauto.
-    eapply link_eval_eq with (Cout := Cout) (bmem := bmem) in ARG; eauto.
-    destruct st_lam. subst inject_C inject_st inject_C' inject_st'.
-    rewrite <- link_update_m_eq; eauto. rewrite lift_plugin_af. rewrite <- plugin_inject_assoc.
-    simpl in *.
-    replace (L _ _ final (tick C (ST mem t) x arg)) with 
-      (link_tick final init Cout α (lift_ctx_bf final init Cout <| lift_ctx_af final init C |>)
-        (ST (link_mem bmem final init Cout mem) (L _ _ final t)) x (inject_ctx_v (lift_ctx_bf final init Cout) (lift_v_af final init arg))).
-    apply (@one_appbody (link final init) _ _ (link_time final init Cout α) 
-                        (lift_ctx_bf _ init Cout <| lift_ctx_af final _ C |>)
-                        (ST (link_mem bmem final init Cout mem0) (L _ _ final t0))
-                        e1 e2 x e (lift_ctx_bf _ init Cout <| lift_ctx_af final _ C_lam |>)
-                        (ST (link_mem bmem final init Cout mem1) (L _ _ final t1))
-                        (inject_ctx_v (lift_ctx_bf _ init Cout) (lift_v_af final _ arg))
-                        (link_mem bmem final init Cout mem) (L _ _ final t)). eauto. eauto.
-    destruct arg. simpl. rewrite t_refl.
-    repeat rewrite delete_inject_eq. repeat rewrite filter_delete_eq. repeat rewrite filter_lift_eq_af. eauto.
-    intros; rewrite eqb_eq; eauto. intros; rewrite eqb_eq; eauto.
-  - apply one_linkl.
-  - destruct st_m.
-    eapply link_eval_eq with (Cout := Cout) (bmem := bmem) in MOD; eauto.
-    eapply one_linkr; simpl in *; eauto.
-  - apply one_letel.
-  - eapply link_eval_eq with (Cout := Cout) (bmem := bmem) in EVALx; eauto.
-    subst inject_C inject_st inject_C' inject_st'.
-    rewrite <- link_update_m_eq; eauto. rewrite lift_plugin_af. rewrite <- plugin_inject_assoc.
-    simpl in *.
-    replace (L _ _ final (tick C (ST mem t) x v)) with 
-      (link_tick final init Cout α (lift_ctx_bf _ init Cout <| lift_ctx_af final _ C |>)
-        (ST (link_mem bmem final init Cout mem) (L _ _ final t)) x (inject_ctx_v (lift_ctx_bf _ init Cout) (lift_v_af final _ v))).
-    apply (@one_leter (link final init) _ _ (link_time final init Cout α) 
-                      (lift_ctx_bf _ init Cout <| lift_ctx_af final _ C |>)
-                      (ST (link_mem bmem final init Cout mem0) (L _ _ final t0))
-                      x e m 
-                      (inject_ctx_v (lift_ctx_bf _ init Cout) (lift_v_af final _ v))
-                      (link_mem bmem final init Cout mem) (L _ _ final t)). eauto.
-    destruct v. simpl. rewrite t_refl.
-    repeat rewrite delete_inject_eq. repeat rewrite filter_delete_eq. repeat rewrite filter_lift_eq_af. eauto.
-    intros; rewrite eqb_eq; eauto. intros; rewrite eqb_eq; eauto.
-  - apply one_letml.
-  - destruct st_M.
-    eapply link_eval_eq with (Cout := Cout) (bmem := bmem) in EVALM; eauto.
-    subst inject_C inject_st inject_C' inject_st'.
-    rewrite lift_plugin_af. rewrite <- plugin_inject_assoc.
-    simpl in *.
-    eapply one_letmr; simpl in *; eauto.
+  intros. remember (Cf e C m t) as cf.
+  ginduction EVAL; ii; ss; repeat des_goal; repeat des_hyp; clarify;
+  match goal with
+  | ADDR : addr_x ?Cin ?x = Some ?addr,
+    ACCESS : read ?m ?addr = Some (Closure ?x_lam ?e ?C)
+    |- context[ (lift_ctx_af ?Cin) [|lift_ctx_bf ?Cout|] ] =>
+    let RR := fresh "RR" in
+    pose proof (inject_addr_x x (lift_ctx_bf Cout) (lift_ctx_af Cin));
+    pose proof (@lift_addr_x BT AT Cin x) as RR;
+    rewrite ADDR in *; rewrite RR in *;
+    assert (Some (Closure x_lam e (lift_ctx_af C [|lift_ctx_bf Cout|])) =
+      read (link_mem bmem Cout m) (AF addr)); 
+    first [
+      unfold link_mem;
+      induction m; ss; repeat des_goal; repeat des_hyp;
+      clarify; eauto | eauto]
+  | ACCESS: ctx_M ?Cin ?M = _
+    |- context [lift_ctx_af ?Cin [|lift_ctx_bf ?Cout|] ] =>
+    let RR := fresh "RR" in
+    pose proof (@lift_ctx_M BT AT Cin M) as RR;
+    pose proof (inject_ctx_M M (lift_ctx_bf Cout) (lift_ctx_af Cin));
+    rewrite ACCESS in *;
+    rewrite RR in *; eauto
+  | _ => solve [exploit (IHEVAL T); eauto]
+  | _ =>
+    let RR := fresh "RR" in
+    let RRR := fresh "RRR" in
+    try (exploit (IHEVAL1 T); eauto; instantiate (1 := Cout); instantiate (1 := bmem); ii);
+    try (exploit (IHEVAL2 T); eauto; instantiate (1 := Cout); instantiate (1 := bmem); ii);
+    try (exploit (IHEVAL3 T); eauto; instantiate (1 := Cout); instantiate (1 := bmem); ii);
+    pose proof (@link_tick_eq T _ BT _ _ _ AT _ _ _ Cout α bmem) as RR;
+    pose proof (@link_update_m_eq BT _ AT _ Cout bmem) as RRR;
+    rewrite <- RRR in *;
+    rewrite <- RR in *;
+    pose proof (@AppBody (link BT AT) _ _ (link_time Cout α));
+    pose proof (@App (link BT AT) _ _ (link_time Cout α));
+    pose proof (@LetER (link BT AT) _ _ (link_time Cout α));
+    pose proof (@LetE (link BT AT) _ _ (link_time Cout α));
+    simpl tick in *;
+    eauto
+  end.
 Qed.
